back to uint as it has easier semantics. adding auto combine/split hints for logicalR. nat has too many missing hints/automation to deal with mod. will switch to N

monadproofs/tutorials/demo2.cpp
@@ -246,3 +246,4 @@ int testgcdl() {
 void incdata(Node * n){
   n->data_++;
 }
+std::atomic<uint> uldkjflkasj;// just to force clang to produce the ast of std::atomic<uint>. there is probably a better way to do it
